Define strongest postcondition and relevant lemmas

Core/LogicFacts.v
@@ -44,21 +44,22 @@ repeat lazymatch goal with
 | [ H : TInvoke ?impl ?i ?A ?l ?s ?ρ ?t ?σ |- ?G ] => destruct H
 | [ H : ReltToPrec ?R ?s ?ρ |- ?G ] => destruct H
 end;
-repeat lazymatch goal with
-| [ H : InterStep ?i ?st ?ev ?st' |- ?G ] => dependent destruction H
-| [ H : Step ?impl ?st ?ev ?st' |- ?G ] => idtac ev; simpl in H; dependent destruction H
-end;
 simpl in *;
 subst;
 repeat lazymatch goal with
 | [ H : ?A, H' : ?A |- ?G] => clear H'
 end.
 
+Ltac steps :=
+repeat match goal with
+| [ H : InterStep ?i ?st ?e ?st' |- ?G ] => dependent destruction H
+| [ H : Step ?impl ?st ?ev ?st' |- ?G ] => simpl in H; dependent destruction H
+end.
 
 Lemma precCompStable {E VE F} {R : @Relt E VE F} {P Q} :
   Stable R P ->
   Stable R Q ->
-  Stable R (P << Q).
+  Stable R (P <<- Q).
 intros.
 unfold Stable, stablePrec, sub, subPrec.
 intros.
@@ -75,7 +76,7 @@ Qed.
 Lemma reltCompStable {E VE F} {R : @Relt E VE F} {Q S} :
   Stable R Q ->
   Stable R S ->
-  Stable R (Q >> S).
+  Stable R (Q ->> S).
 intros.
 unfold Stable, stableRelt, sub, subRelt.
 split.
@@ -104,7 +105,7 @@ Qed.
 Lemma reltStableHelp {E VE F} {R : @Relt E VE F} {Q} :
     Stable R Q ->
     forall s ρ t σ,
-    (((R >> Q) s ρ t σ) \/ ((Q >> R) s ρ t σ)) ->
+    (((R ->> Q) s ρ t σ) \/ ((Q ->> R) s ρ t σ)) ->
     Q s ρ t σ.
 intros.
 destruct H.
@@ -115,7 +116,7 @@ apply H1.
 easy.
 Qed.
 
-Lemma rtcTrans {E VE F} {R : Relt E VE F} : (RTC R >> RTC R) ==> RTC R.
+Lemma rtcTrans {E VE F} {R : Relt E VE F} : (RTC R ->> RTC R) ==> RTC R.
 unfold sub, subRelt.
 intros.
 pdestruct H.
@@ -128,8 +129,8 @@ easy.
 Qed.
 
 Lemma precStabilizedStable {E VE F} {R : Relt E VE F} {P} :
-  (R >> R ==> R) ->
-  Stable R (P << R).
+  (R ->> R ==> R) ->
+  Stable R (P <<- R).
 intros.
 unfold Stable, stablePrec, sub, subPrec.
 intros.
@@ -159,11 +160,11 @@ Qed.
 
 Ltac stable :=
 lazymatch goal with
-| [ H : ?R >> ?R ==> ?R |- @Stable _ _ _ _ stableRelt ?R (?P << ?R) ] =>
+| [ H : ?R ->> ?R ==> ?R |- @Stable _ _ _ _ stableRelt ?R (?P <<- ?R) ] =>
     apply (precStabilizedStable H)
-| [ |- @Stable _ _ _ _ stablePrec ?R (?P << ?Q) ] =>
+| [ |- @Stable _ _ _ _ stablePrec ?R (?P <<- ?Q) ] =>
     eapply precCompStable; stable
-| [ |- @Stable _ _ _ _ stableRelt ?R (?Q >> ?S) ] =>
+| [ |- @Stable _ _ _ _ stableRelt ?R (?Q ->> ?S) ] =>
     eapply reltCompStable; stable
 | [ H : @Stable _ _ _ _ stablePrec ?R ?P |- ?P ?s ?ρ ] =>
     apply H
@@ -186,8 +187,8 @@ constructor.
 apply rt_refl.
 Qed.
 
-Lemma safeBind {E F VF VE impl i R G P A B} {S : Post E VE F B} {m : E A} {k : A -> Prog E B} :
-  forall QI QR,
+(* Lemma safeBind {E F VF VE impl i R G P A B} {S : Post E VE F B} {m : E A} {k : A -> Prog E B} :
+  forall PR PK,
   Stable R QI ->
   Commit VF i impl G P (CallEv m) QI ->
   Stable R QR ->
@@ -202,20 +203,184 @@ exact H.
 exact H1.
 easy.
 easy.
+Qed. *)
+
+Create HintDb rely_lemmas.
+
+Definition sp {E VE F} impl i VF (R : Relt E VE F) (P : Prec E VE F) ev : Relt E VE F :=
+  fun s ρ t σ =>
+    exists rs rρ,
+      R s ρ rs rρ /\
+      P rs rρ /\
+      exists rt rσ,
+        InterStep (impl:=impl) i rs (i, liftUEv ev) rt /\
+        IsTraceOfSpec rσ VF /\
+        LinRw rρ rσ /\
+        R rt rσ t σ.
+
+Lemma spStrongest E VE F VF impl i (R G : Relt E VE F) P ev :
+  id ==> R ->
+  sp impl i VF R P ev ==> G ->
+  Commit VF i impl G P ev (sp impl i VF R P ev).
+intros Rid Gsub.
+unfold Commit, sp.
+intros.
+do 2 destruct H.
+exists x.
+split.
+do 2 eexists.
+split.
+apply Rid.
+unfold id.
+easy.
+split.
+easy.
+do 2 eexists.
+split.
+exact H1.
+split.
+exact H.
+split.
+easy.
+apply Rid.
+unfold id.
+easy.
+split.
+apply Gsub.
+unfold sp.
+do 2 eexists.
+split.
+apply Rid.
+unfold id.
+easy.
+split.
+easy.
+do 2 eexists.
+split.
+exact H1.
+split.
+exact H.
+split.
+easy.
+apply Rid.
+unfold id.
+easy.
+exists nil.
+split.
+constructor.
+rewrite app_nil_r.
+easy.
 Qed.
 
-(* Lemma safeBindAcc {E F VF VE impl i R G P A B} {S : Post E VE F B} {m : E A} {k : A -> Prog E B} :
-  forall QI QR,
-  Stable R QI ->
-  Commit VF i impl R G P (CallEv m) QI ->
-  Stable R QR ->
-  (forall v,
-    Commit VF i impl R G (P << QI) (RetEv m v) QR /\
-    VerifyProg VF i impl R G (P << QI << QR) (k v) S) ->
-  VerifyProg VF i impl R G P (Bind m k) S.
+Lemma spStable E VE F VF impl i (R : Relt E VE F) P ev :
+  R ->> R ==> R ->
+  Stable R (sp impl i VF R P ev).
+intros Rtrans.
+unfold Stable, stableRelt, sub, subRelt, sp.
+split.
 intros.
-eapply safeBind. *)
+{
+  psimpl.
+  do 2 eexists.
+  split.
+  apply Rtrans.
+  psplit.
+  exact H.
+  exact H0.
+  split.
+  easy.
+  do 2 eexists.
+  split.
+  exact H2.
+  split.
+  exact H3.
+  easy.
+}
+{
+  intros.
+  psimpl.
+  do 2 eexists.
+  split.
+  exact H.
+  split.
+  easy.
+  do 2 eexists.
+  split.
+  exact H2.
+  split.
+  exact H3.
+  split.
+  easy.
+  apply Rtrans.
+  psplit.
+  exact H5.
+  easy.
+}
+Qed.
 
+Lemma strongBind {E F VF VE impl i R G P A B} {S : Post E VE F B} {m : E A} {k : A -> Prog E B} :
+  id ==> R ->
+  R ->> R ==> R ->
+  sp impl i VF R P (CallEv m) ==> G ->
+  (forall v,
+    sp impl i VF R (sp impl i VF R P (CallEv m)) (RetEv m v) ==> G) ->
+  (forall v,
+    VerifyProg VF i impl R G
+      (sp impl i VF R
+        (sp impl i VF R P (CallEv m)) (RetEv m v))
+      (k v)
+      S) ->
+  VerifyProg VF i impl R G P (Bind m k) S.
+intros Rid Rtrans Gsub1 Gsub2. intros.
+apply SafeBind with
+  (QI:= sp impl i VF R P (CallEv m))
+  (QR:= fun v => sp impl i VF R (sp impl i VF R P (CallEv m)) (RetEv m v)).
+apply spStable.
+easy.
+unfold Stable, stablePost.
+intros.
+apply spStable.
+easy.
+apply spStrongest.
+easy.
+easy.
+intros.
+split.
+apply spStrongest.
+easy.
+easy.
+apply H.
+Qed.
+
+Ltac strongBind := eapply strongBind; eauto with rely_lemmas.
+
+Axiom undef : forall a, a.
+
+Lemma weakenPrec E F A VE VF i impl (R : Relt E VE F) G P P' Q (C : Prog E A) :
+  VerifyProg VF i impl R G P C Q ->
+  P' ==> P ->
+  VerifyProg VF i impl R G P' C Q.
+intros.
+destruct C.
+dependent destruction H.
+apply SafeBind with (QI:=QI) (QR:=QR).
+easy.
+easy.
+unfold Commit.
+intros.
+apply H1.
+easy.
+apply H3.
+easy.
+easy.
+easy.
+dependent destruction H.
+constructor.
+intros.
+apply H.
+apply H0.
+easy.
+Admitted.
 
 Theorem soundness {E F} (lay : Layer E F) VF :
   (exists R G P Q, VerifyImpl lay.(USpec) VF R G P lay.(LImpl) Q) ->
